Merge conflicts on SBisim solved
- Define sbisim in terms of the heterogenous version
- Modify symemtry proofs to use ltac automation instead
- Some admitted lemmas still

theories/Eq/SBisim.v
@@ -40,7 +40,12 @@ answered by [wtrans].
 
 .. coq::none
 |*)
-From Coq Require Import Lia Basics Fin.
+From Coq Require Import
+     Lia
+     Basics
+     Fin
+     Program.Equality
+     Logic.Eqdep.
 
 From Coinduction Require Import
      coinduction rel tactics.
@@ -108,7 +113,7 @@ Complete strong simulation [ss].
 
 End StrongSim.
 
-Section StrongHBisim.
+Section StrongSBisim.
   Context {E F C D : Type -> Type} {X Y : Type} `{HasStuck : B0 -< C} `{HasStuck' : B0 -< D}.
   Notation S := (ctree E C X).
   Notation S' := (ctree F D Y).
@@ -116,23 +121,13 @@ Section StrongHBisim.
 (*|
 In the heterogeneous case, the relation is not symmetric.
 |*)
-  Program Definition hsb L : mon (S -> S' -> Prop) :=
+  Program Definition sb L : mon (S -> S' -> Prop) :=
     {| body R t u := ss0 L R t u /\ ss0 (flip L) (flip R) u t |}.
   Next Obligation.
     split; intros; [edestruct H0 as (? & ? & ?) | edestruct H1 as (? & ? & ?)]; eauto; eexists; eexists; intuition; eauto.
   Qed.
 
-End StrongHBisim.
-
-(*|
-Define `sb` in terms of `hsb`
-|*)
-Section StrongBisim.
-  Context {E C : Type -> Type} {X : Type} `{HasStuck' : B0 -< C}.
-  Notation S := (ctree E C X).
-
-  Definition sb L : mon (S -> S -> Prop) := hsb L.
-End StrongBisim.
+End StrongSBisim.
 
 (*|
 The relations themselves
@@ -144,10 +139,8 @@ Definition ssim0 {E F C D X Y} `{HasStuck : B0 -< C} `{HasStuck' : B0 -< D} L :=
 Definition ssim {E F C D X Y} `{HasStuck : B0 -< C} `{HasStuck' : B0 -< D} L :=
   (gfp (@ss E F C D X Y _ _ L) : hrel _ _).
 
-Definition sbisim {E C X} `{HasStuck : B0 -< C} L := (gfp (@sb E C X _ L) : hrel _ _).
-
-Definition hsbisim {E F C D X Y} `{HasStuck : B0 -< C} `{HasStuck' : B0 -< D} L :=
-  (gfp (@hsb E F C D X Y _ _ L) : hrel _ _).
+Definition sbisim {E F C D X Y} `{HasStuck : B0 -< C} `{HasStuck': B0 -< D} L :=
+  (gfp (@sb E F C D X Y _ _ L) : hrel _ _).
 
 Module SBisimNotations.
 
@@ -197,8 +190,6 @@ Import SBisimNotations.
 Ltac fold_sbisim :=
   repeat
     match goal with
-    | h: context[gfp (@hsb ?E ?F ?C ?D ?X ?Y _ _ ?L)] |- _ => fold (@hsbisim E F C D X Y _ _ L) in h
-    | |- context[gfp (@hsb ?E ?F ?C ?D ?X ?Y _ _ ?L)]      => fold (@hsbisim E F C D X Y _ _ L)
     | h: context[gfp (@sb ?E ?C ?X _)] |- _ => fold (@sbisim E C X _) in h
     | |- context[gfp (@sb ?E ?C ?X _)]      => fold (@sbisim E C X _)
     | h: context[gfp (@ss ?E ?F ?C ?D ?X ?Y _ _ ?L)] |- _ => fold (@ssim E F C D X Y _ _ L) in h
@@ -209,7 +200,6 @@ Ltac fold_sbisim :=
 
 Ltac __coinduction_sbisim R H :=
   (try unfold sbisim);
-  (try unfold hsbisim);
   (try unfold ssim0);
   (try unfold ssim);
   apply_coinduction; fold_sbisim; intros R H.
@@ -228,14 +218,6 @@ Tactic Notation "__step_sbisim" :=
       unfold ss;
       step;
       fold (@ss E F C D X Y _ _ LR)
-  | |- context[@hsbisim ?E ?F ?C ?D ?X ?Y _ _ ?LR] =>
-      unfold hsbisim;
-      step;
-      fold (@hsbisim E F C D X Y _ _ LR)
-  | |- context[@hsb ?E ?F ?C ?D ?X ?Y _ _ ?LR] =>
-      unfold hsb;
-      step;
-      fold (@hsb E F C D X Y _ _ LR)
   | |- context[@sbisim ?E ?C ?X _] =>
       unfold sbisim;
       step;
@@ -261,10 +243,6 @@ Ltac __step_in_sbisim H :=
       unfold ssim in H;
       step in H;
       fold (@ssim E F C D X Y _ _ LR) in H
-  | context[@hsbisim ?E ?F ?C ?D ?X ?Y _ _ ?LR] =>
-      unfold hsbisim in H;
-      step in H;
-      fold (@hsbisim E F C D X Y _ _ LR) in H
   | context [@sbisim ?E ?C ?X _] =>
       unfold sbisim in H;
       step in H;
@@ -274,65 +252,26 @@ Ltac __step_in_sbisim H :=
 #[local] Tactic Notation "step" "in" ident(H) := __step_in_sbisim H || step in H.
 
 (*|
-The two definitions of homogeneous bisimulation are equivalent.
-|*)
-Lemma hsbisim_eq_sbisim : forall {E C X} `{B0 -< C} L (t t' : ctree E C X),
-  hsbisim L t t' <-> sbisim L t t'.
-Proof.
-  split; intros; revert t t' H0;
-    coinduction R CH; intros; step in H0; cbn in H0;
-    split; cbn; intros; apply H0 in H1 as (? & ? & ? & ? & ?); subst;
-    exists x, x0; split; auto.
-Qed.
-
-(*|
 A bisimulation trivially gives a simulation.
 |*)
-Lemma hsb_ss : forall {E F C D X Y} `{B0 -< C} `{B0 -< D} L RR
+Lemma sb_ss : forall {E F C D X Y} `{B0 -< C} `{B0 -< D} L RR
   (t : ctree E C X) (t' : ctree F D Y),
-  hsb L RR t t' -> ss L RR t t'.
+  sb L RR t t' -> ss L RR t t'.
 Proof.
   intros; split.
   - apply H1.
   - intros. apply H1 in H2 as (? & ? & ? & ? & ?). eauto.
 Qed.
 
-Lemma hsbisim_ssim : forall {E F C D X Y} `{B0 -< C} `{B0 -< D} L
+Lemma sbisim_ssim : forall {E F C D X Y} `{B0 -< C} `{B0 -< D} L
   (t : ctree E C X) (t' : ctree F D Y),
-  hsbisim L t t' -> ssim L t t'.
+  sbisim L t t' -> ssim L t t'.
 Proof.
   intros until L.
   coinduction R CH. simpl. intros.
   split; step in H1; intros;
     apply H1 in H2 as (? & ? & ? & ? & ?);
     exists x, x0; auto.
-Qed.
-
-Lemma sbisim_ssim_eq : forall {E C X} `{B0 -< C} (t t' : ctree E C X) L,
-  sbisim L t t' -> ssim L t t'.
-Proof.
-  intros. apply hsbisim_eq_sbisim in H0.
-  now apply hsbisim_ssim in H0 as H1.
-Qed.
-
-Lemma sb_ss : forall {E C X} `{B0 -< C} RR L (t t' : ctree E C X),
-  sb L RR t t' -> ss L RR t t'.
-Proof.
-  intros. split.
-  - apply H0.
-  - intros; apply H0 in H1 as (? & ? & ? & ? & ?); eauto.
-Qed.
-
-Lemma sbisim_ssim : forall
-    {E C X} `{B0 -< C} L (t t' : ctree E C X),
-  sbisim L t t' -> ssim L t t'.
-Proof.
-  intros until L.
-  coinduction R CH; simpl; intros.
-  step in H0; split; intros;
-    apply H0 in H1 as (? & ? & ? & ? & ?);
-    exists x, x0; split; try assumption;
-    apply H0 in H1 as (? & ? & ? & ? & ?); split; eauto.
 Qed.
 
 Lemma ssim_ssim0 : forall {E C X} `{B0 -< C} L (t t' : ctree E C X),
@@ -352,37 +291,58 @@ Proof.
   intros. apply ssim_ssim0. now apply sbisim_ssim.
 Qed.
 
-Section sbisim_theory.
+Section sbisim_heterogenous_theory.
+  Notation hss E F C D X Y L := (@ss E F C D X Y _ _ L).
+  Notation hsb E F C D X Y L := (@sb E F C D X Y _ _ L).
+  Notation hsbisim E F C D X Y L := (@sbisim E F C D X Y _ _ L).
 
-  Context {E C : Type -> Type} {X : Type} `{HasStuck : B0 -< C}.
+  Notation ss E C X := (@ss E E C C X X _ _ eq).
+  Notation sb E C X := (@sb E E C C X X _ _ eq).
+  Notation sbisim E C X:= (@sbisim E E C C X X _ _ eq).
+  
+  Notation st  E C X := (coinduction.t (sb E C X)).
+  Notation sbt E C X := (coinduction.bt (sb E C X)).
+  Notation sT  E C X := (coinduction.T (sb E C X)).
+
+  #[global] Instance sbisim_sbisim_hclosed_goal {E F C D: Type -> Type} {X Y: Type}
+   `{HasStuck1 : B0 -< C} `{HasStuck2 : B0 -< D} {L: rel (@label E) (@label F)} :
+    
+    Proper (sbisim E C X ==> sbisim F D Y ==> flip impl)
+           (hsbisim E F C D X Y L).
+  Admitted.
+
+  
+End sbisim_heterogenous_theory.
+
+Section sbisim_homogenous_theory.
+  Context {E C: Type -> Type} {X: Type} `{HasStuck: B0 -< C}.
   Notation ss := (@ss E E C C X X _ _ eq).
-  Notation sb := (@sb E C X _ eq).
-  Notation sbisim := (@sbisim E C X _ eq).
+  Notation sb  := (@sb E E C C X X _ _ eq).
+  Notation sbisim := (@sbisim E E C C X X _ _ eq).
+
   Notation st := (coinduction.t sb).
   Notation sbt := (coinduction.bt sb).
-  Notation sT := (coinduction.T sb).
-(*|
-This is just a hack suggested by Damien Pous to avoid a
-universe inconsistency when using both the relational algebra
-and coinduction libraries (we fix the type at which we'll use [eq]).
-|*)
-    Definition seq: relation (ctree E C X) := eq.
-    Arguments seq/.
+  Notation sT  := (coinduction.T sb).
 
-(*|
-[eq] is a post-fixpoint, thus [const eq] is below [t]
-i.e. validity of up-to reflexivity
-|*)
+  (*|
+    This is just a hack suggested by Damien Pous to avoid a
+    universe inconsistency when using both the relational algebra
+    and coinduction libraries (we fix the type at which we'll use [eq]).
+    |*)
+  Definition seq: relation (ctree E C X) := eq.
+  Arguments seq/.
+
   Lemma refl_st : const seq <= st.
   Proof.
     apply leq_t.
-    split; intros; cbn*; intros; inv H; subst; exists l, t'; split; eauto.
+    split; intros; cbn*; intros; inv H; subst;
+      exists l, t'; split; eauto.
   Qed.
 
-(*|
-[converse] is compatible
-i.e. validity of up-to symmetry
-|*)
+  (*|
+    [converse] is compatible
+    i.e. validity of up-to symmetry
+    |*)
   Lemma converse_st: converse <= st.
   Proof.
     apply leq_t; cbn.
@@ -391,10 +351,10 @@ i.e. validity of up-to symmetry
     - destruct (H1 _ _ H) as (? & ? & ? & ? & ?); subst; eauto.
   Qed.
 
-(*|
-[square] is compatible
- i.e. validity of up-to transivitiy
-|*)
+  (*|
+    [square] is compatible
+    i.e. validity of up-to transivitiy
+    |*)
   Lemma square_st: square <= st.
   Proof.
     apply Coinduction; cbn.    
@@ -414,9 +374,9 @@ i.e. validity of up-to symmetry
       eexists; eauto.
   Qed.
 
-(*|
-Thus bisimilarity and [t R] are always equivalence relations.
-|*)
+  (*|
+    Thus bisimilarity and [t R] are always equivalence relations.
+    |*)
   #[global] Instance Equivalence_st R: Equivalence (st R).
   Proof. apply Equivalence_t. apply refl_st. apply square_st. apply converse_st. Qed.
 
@@ -429,7 +389,7 @@ Thus bisimilarity and [t R] are always equivalence relations.
   #[global] Instance Equivalence_sT f R: Equivalence ((T sb) f R).
   Proof. apply rel.Equivalence_T. apply refl_st. apply square_st. apply converse_st. Qed.
 
-(*|
+  (*|
 Aggressively providing instances for rewriting hopefully faster
 [sbisim] under all [sb]-related contexts (consequence of the transitivity
 of the companion).
@@ -479,18 +439,17 @@ of the companion).
     auto.
   Qed.
 
-(*|
-Strong bisimulation up-to [equ] is valid
-----------------------------------------
-|*)
+  (*|
+    Strong bisimulation up-to [equ] is valid
+    ----------------------------------------
+    |*)
   Lemma equ_clos_st : equ_clos <= st.
   Proof.
     apply Coinduction; cbn.
-    intros R x y [x' y' x'' y'' EQ' [? ?] EQ'']; split.
-    - intros l z x'z.
-  Admitted.
-  (*
-    apply equ_clos_sym.
+    intros R x1 y1 [x2 y2 x3 y3 EQ2 [H1 H2] EQ3].
+    split; intros; cbn*.
+    Admitted.
+  (* apply equ_clos_sym.
     intros R t u EQ l t1 TR. cbn in EQ. inv EQ.
     destruct HR as [F _]; cbn in *.
     rewrite Equt in TR.
@@ -501,13 +460,13 @@ Strong bisimulation up-to [equ] is valid
     eapply (f_Tf sb).
     econstructor; intuition.
     auto.
-  Qed.
-*)
+  Qed. *)
+  
 
-(*|
-Aggressively providing instances for rewriting [equ] under all [sb]-related
-contexts.
-|*)
+  (*|
+    Aggressively providing instances for rewriting [equ] under all [sb]-related
+    contexts.
+    |*)
   #[global] Instance equ_clos_st_goal RR :
     Proper (equ eq ==> equ eq ==> flip impl) (st RR).
   Proof.
@@ -594,7 +553,7 @@ contexts.
     rewrite tt', uu'. reflexivity.
   Qed.
 
-(*|
+  (*|
 Hence [equ eq] is a included in [sbisim]
 |*)
   #[global] Instance equ_sbisim_subrelation : subrelation (equ eq) sbisim.
@@ -602,9 +561,7 @@ Hence [equ eq] is a included in [sbisim]
     red; intros.
     rewrite H; reflexivity.
   Qed.
-
-End sbisim_theory.
-
+End sbisim_homogenous_theory.
 
 (* Up-to-bisimulation enhancing function *)
 Variant sbisim_clos_body {E F C D X1 X2} `{B0 -< C} `{B0 -< D} (R : rel (ctree E C X1) (ctree F D X2)) : (rel (ctree E C X1) (ctree F D X2)) :=
@@ -629,16 +586,14 @@ a valid enhancement to prove [equ].
 We now prove the same result, but for strong and weak bisimulation.
 |*)
 
-Section bind.
-  Obligation Tactic := idtac.
-
- Context {E C: Type -> Type} {X Y: Type} `{HasStuck : B0 -< C}.
-
-(*|
-Specialization of [bind_ctx] to a function acting with [sisim] on the bound value,
-and with the argument (pointwise) on the continuation.
-|*)
- (* LEF: TODO heterogeneous? *)
+Section bind_homogenous.
+  Obligation Tactic := trivial.
+  Context {E C: Type -> Type} {X Y: Type} `{HasStuck: B0 -< C}.
+   
+  (*|
+    Specialization of [bind_ctx] to a function acting with [hsisim] on the bound value,
+    and with the argument (pointwise) on the continuation.
+    |*)
   Program Definition bind_ctx_sbisim : mon (rel (ctree E C Y) (ctree E C Y)) :=
     {|body := fun R => @bind_ctx E E C C X X Y Y (sbisim eq) (pointwise eq R) |}.
   Next Obligation.
@@ -646,9 +601,9 @@ and with the argument (pointwise) on the continuation.
     apply in_bind_ctx. apply H'. intros t t' HS. apply H, H'', HS.
   Qed.
 
-(*|
-Sufficient condition to exploit symmetry
-|*)
+  (*|
+    Sufficient condition to exploit symmetry
+    |*)
   Lemma bind_ctx_sbisim_sym: compat converse bind_ctx_sbisim.
   Proof.
     intro R. simpl. apply leq_bind_ctx. intros. apply in_bind_ctx.
@@ -657,15 +612,18 @@ Sufficient condition to exploit symmetry
     apply H0; auto.
   Qed.
 
-  (* LEF: Up to here *)
-(*|
-The resulting enhancing function gives a valid up-to technique
-|*)
+  (*|
+    The resulting enhancing function gives a valid up-to technique
+    |*)
   Lemma bind_ctx_sbisim_t : bind_ctx_sbisim <= (st eq).
   Proof.
-    apply Coinduction, by_Symmetry.
+    apply Coinduction; cbn.
+    
+    intros R x y [z _ [t zt [k1 _ [k2 EQ]]]]; inv H; split; intros.
+    - edestruct EQ; trivial. 
+      (*
     apply bind_ctx_sbisim_sym.
-    intros R. apply (leq_bind_ctx _).
+    intros R. 
     intros t1 t2 tt k1 k2 kk.
     step in tt; destruct tt as (F & B); cbn in *.
     cbn in *; intros l u STEP.
@@ -689,9 +647,10 @@ The resulting enhancing function gives a valid up-to technique
       eapply trans_bind_r; cbn in *; eauto.
       split; auto.
       eapply (id_T sb); cbn; auto.
-  Qed.
+       *)
+  Admitted.
 
-End bind.
+End bind_homogenous.
 
 Import CTree.
 Import CTreeNotations.
@@ -702,8 +661,8 @@ Expliciting the reasoning rule provided by the up-to principles.
 Lemma st_clo_bind (E C: Type -> Type) `{B0 -< C} (X Y : Type) :
 	forall (t1 t2 : ctree E C X) (k1 k2 : X -> ctree E C Y) RR,
 		t1 ~ t2 ->
-    (forall x, (st RR) (k1 x) (k2 x)) ->
-    st RR (t1 >>= k1) (t2 >>= k2)
+    (forall x, (st eq RR) (k1 x) (k2 x)) ->
+    st eq RR (t1 >>= k1) (t2 >>= k2)
 .
 Proof.
   intros.
@@ -734,7 +693,7 @@ And in particular, we get the proper instance justifying rewriting [~] to the le
 |*)
 #[global] Instance bind_sbisim_cong_gen :
  forall (E C : Type -> Type) `{B0 -< C} (X Y : Type) RR,
-   Proper (sbisim ==> pointwise_relation X (st RR) ==> st RR) (@bind E C X Y).
+   Proper (sbisim eq ==> pointwise_relation X (st eq RR) ==> st eq RR) (@bind E C X Y).
 Proof.
   repeat red; intros; eapply st_clo_bind; eauto.
 Qed.
@@ -800,7 +759,7 @@ Section sb_vis_ctx.
 (*|
 The resulting enhancing function gives a valid up-to technique
 |*)
-  Lemma vis_ctx_sbisim_t `{B0 -< C} (e : E X) : vis_ctx_sbisim e <= st.
+  Lemma vis_ctx_sbisim_t `{B0 -< C} (e : E X) : vis_ctx_sbisim e <= (st eq).
   Proof.
     apply Coinduction.
     intros R.
@@ -813,7 +772,7 @@ The resulting enhancing function gives a valid up-to technique
     all: split; auto.
     all: rewrite EQ.
     all: specialize (kk' x x eq_refl).
-    all: now eapply (b_T sb).
+    all: now eapply (b_T (sb eq)).
   Qed.
 
 End sb_vis_ctx.
@@ -821,10 +780,11 @@ Arguments vis_ctx_sbisim_t {_ _ _ _ _} e.
 
 Ltac __upto_vis_sbisim :=
   match goal with
-    |- @sbisim _ _ ?X _ (Vis ?e _) (Vis ?e _) => apply (ft_t (vis_ctx_sbisim_t (Y := X) e)), in_vis_ctx; intros ? ? <-
-  | |- body (t (@sb ?E ?C ?R _)) ?RR (Vis ?e _) (Vis ?e _) =>
+    |- @sbisim ?E _ ?C _ ?X _ _ _ ?RR (Vis ?e _) (Vis ?e _) =>
+      apply (ft_t (vis_ctx_sbisim_t (Y := X) e)), in_vis_ctx; intros ? ? <-
+  | |- body (t (@sb ?E _ ?C _ ?X _ _ ?R _)) ?RR (Vis ?e _) (Vis ?e _) =>
       apply (ft_t (vis_ctx_sbisim_t e)), in_vis_ctx; intros ? ? <-
-  | |- body (bt (@sb ?E ?C ?R _)) ?RR (Vis ?e _) (Vis ?e _) =>
+  | |- body (bt (@sb ?E _ ?C _ ?X _ _ ?R _)) ?RR (Vis ?e _) (Vis ?e _) =>
       apply (fbt_bt (vis_ctx_sbisim_t e)), in_vis_ctx; intros ? ? <-
   end.
 
@@ -836,21 +796,12 @@ Ltac __playL_sbisim H :=
   step in H;
   let Hf := fresh "Hf" in
   destruct H as [Hf _];
-<<<<<<< HEAD
   cbn in Hf; edestruct Hf as (? & ? & ?TR & ?EQ & ?);
   clear Hf; subst; [etrans |].
 
 Ltac __eplayL_sbisim :=
   match goal with
-  | h : @sbisim ?E ?C ?X _ _ _ |- _ =>
-=======
-  cbn in Hf; edestruct Hf as [? ?TR ?EQ];
-  clear Hf; [etrans |].
-
-Ltac __eplayL_sbisim :=
-  match goal with
-  | h : @sbisim ?E ?X _ _ |- _ =>
->>>>>>> master
+  | h : @sbisim ?E _ ?C _ ?X _ _ _ ?RR _ _ |- _ =>
       __playL_sbisim h
   end.
 
@@ -858,21 +809,12 @@ Ltac __playR_sbisim H :=
   step in H;
   let Hb := fresh "Hb" in
   destruct H as [_ Hb];
-<<<<<<< HEAD
   cbn in Hb; edestruct Hb as (? & ? & ?TR & ?EQ & ?);
   clear Hb; subst; [etrans |].
 
 Ltac __eplayR_sbisim :=
   match goal with
   | h : @sbisim ?E ?C ?X _ _ _ |- _ =>
-=======
-  cbn in Hb; edestruct Hb;
-  clear Hb; [etrans |].
-
-Ltac __eplayR_sbisim :=
-  match goal with
-  | h : @sbisim ?E ?X _ _ |- _ =>
->>>>>>> master
       __playR_sbisim h
   end.
 
@@ -889,7 +831,7 @@ Naive bisimulations proofs naturally degenerate into exponential proofs,
 splitting into two goals at each step.
 The following proof rules avoid this issue in particular cases.
 
-Be sure to notice that contrary to equations such that [sb_tauI] or
+Be sure to notice that contrary to equations such that [sb_guard] or
 up-to principles such that [upto_vis], (most of) these rules consume a [sb].
 
 TODO: need to think more about this --- do we want more proof rules?
@@ -898,31 +840,27 @@ Do we actually need them on [sb (st R)], or something else?
 
 Section Proof_Rules.
 
-<<<<<<< HEAD
   Context {E C : Type -> Type}.
   Context {HasStuck : B0 -< C}.
-  Context {HasTau : C1 -< C}.
+  Context {HasTau : B1 -< C}.
   Context {X Y : Type}.
+  Context {L: relation (@label E)}.
 
   Lemma step_sb_ret_gen (x y : X) (R : rel _ _) :
-    R stuckI stuckI ->
-=======
-  Lemma step_sb_ret_gen E X (x y : X) (R : rel _ _) :
     R stuckD stuckD ->
->>>>>>> master
     (Proper (equ eq ==> equ eq ==> impl) R) ->
     x = y ->
-    sb R (Ret x) (Ret y : ctree E C X).
+    sb eq R (Ret x) (Ret y : ctree E C X).
   Proof.
     intros Rstuck PROP <-.
     split; cbn; intros ? ? TR; inv_trans; subst.
-    all: cbn; exists stuckI; eexists; intuition; etrans.
+    all: cbn; exists (val x), stuckD; eexists; intuition; etrans.
     all: now rewrite EQ.
   Qed.
 
   Lemma step_sb_ret (x y : X) (R : rel _ _) :
     x = y ->
-    sbt R (Ret x) (Ret y : ctree E C X).
+    sbt eq R (Ret x) (Ret y : ctree E C X).
   Proof.
     apply step_sb_ret_gen.
     reflexivity.
@@ -936,7 +874,7 @@ stepping is hence symmetric and we can just recover the itree-style rule.
   Lemma step_sb_vis_gen (e : E X) (k k' : X -> ctree E C Y) (R : rel _ _) :
     (Proper (equ eq ==> equ eq ==> impl) R) ->
     (forall x, R (k x) (k' x)) ->
-    sb R (Vis e k) (Vis e k').
+    sb eq R (Vis e k) (Vis e k').
   Proof.
     intros PR EQs.
     split; intros ? ? TR; inv_trans; subst.
@@ -944,255 +882,153 @@ stepping is hence symmetric and we can just recover the itree-style rule.
   Qed.
 
   Lemma step_sb_vis (e : E X) (k k' : X -> ctree E C Y) (R : rel _ _) :
-    (forall x, (st R) (k x) (k' x)) ->
-    sbt R (Vis e k) (Vis e k').
+    (forall x, (st eq R) (k x) (k' x)) ->
+    sbt eq R (Vis e k) (Vis e k').
   Proof.
     intros * EQ.
     apply step_sb_vis_gen; auto.
     typeclasses eauto.
   Qed.
 
-(*|
-Same goes for visible tau nodes.
-|*)
-<<<<<<< HEAD
-   Lemma step_sb_tauV_gen (t t' : ctree E C X) (R : rel _ _) :
+  (*|
+    Same goes for visible tau nodes.
+    |*)
+  Lemma step_sb_step_gen (t t' : ctree E C X) (R : rel _ _) :
     (Proper (equ eq ==> equ eq ==> impl) R) ->
     (R t t') ->
-    sb R (tauV t) (tauV t').
-=======
-   Lemma step_sb_step_gen E X (t t' : ctree E X) (R : rel _ _) :
-    (Proper (equ eq ==> equ eq ==> impl) R) ->
-    (R t t') ->
-    sb R (Step t) (Step t').
->>>>>>> master
+    sb eq R (Step t) (Step t').
   Proof.
     intros PR EQs.
     split; intros ? ? TR; inv_trans; subst.
     all: cbn; eexists; eexists; intuition; etrans; rewrite EQ; auto.
   Qed.
 
-<<<<<<< HEAD
-  Lemma step_sb_tauV (t t' : ctree E C X) (R : rel _ _) :
-    (st R t t') ->
-    sbt R (tauV t) (tauV t').
-=======
-  Lemma step_sb_step E X (t t' : ctree E X) (R : rel _ _) :
-    (st R t t') ->
-    sbt R (Step t) (Step t').
->>>>>>> master
+  Lemma step_sb_step (t t' : ctree E C X) (R : rel _ _) :
+    (st eq R t t') ->
+    sbt eq R (Step t) (Step t').
   Proof.
     apply step_sb_step_gen.
     typeclasses eauto.
   Qed.
 
-(*|
-When matching visible brs one against another, in general we need to explain how
-we map the branches from the left to the branches to the right, and reciprocally.
-A useful special case is the one where the arity coincide and we simply use the identity
-in both directions. We can in this case have [n] rather than [2n] obligations.
-|*)
-
-<<<<<<< HEAD
-  Lemma step_sb_choiceV_gen Z (c : C Y) (c' : C Z) (k : Y -> ctree E C X) (k' : Z -> ctree E C X) (R : rel _ _) :
+  (*|
+    When matching visible brs one against another, in general we need to explain how
+    we map the branches from the left to the branches to the right, and reciprocally.
+    A useful special case is the one where the arity coincide and we simply use the identity
+    in both directions. We can in this case have [n] rather than [2n] obligations.
+    |*)
+  Lemma step_sb_brS_gen Z (c : C Y) (c' : C Z) (k : Y -> ctree E C X) (k' : Z -> ctree E C X) (R : rel _ _) :
     (Proper (equ eq ==> equ eq ==> impl) R) ->
     (forall x, exists y, R (k x) (k' y)) ->
     (forall y, exists x, R (k x) (k' y)) ->
-    sb R (ChoiceV c k) (ChoiceV c' k').
-  Proof.
-    intros PROP EQs1 EQs2.
-    split; intros ? ? TR; inv_trans; subst.
-    - destruct (EQs1 x) as [z HR].
-      eexists. eexists. intuition.
-      etrans.
-      rewrite EQ; eauto.
-    - destruct (EQs2 x) as [y HR].
-      eexists. eexists. intuition.
-=======
-  Lemma step_sb_brS_gen E X n m (k : fin n -> ctree E X) (k' : fin m -> ctree E X) (R : rel _ _) :
-    (Proper (equ eq ==> equ eq ==> impl) R) ->
-    (forall x, exists y, R (k x) (k' y)) ->
-    (forall y, exists x, R (k x) (k' y)) ->
-    sb R (BrS n k) (BrS m k').
+    sb eq R (BrS c k) (BrS c' k').
   Proof.
     intros PROP EQs1 EQs2.
     split; intros ? ? TR; inv_trans; subst.
     - destruct (EQs1 x) as [y HR].
-      eexists.
+      eexists. eexists. intuition.
       etrans.
       rewrite EQ; eauto.
     - destruct (EQs2 x) as [y HR].
-      eexists.
->>>>>>> master
+      eexists. eexists. intuition.
       etrans.
       cbn; rewrite EQ; eauto.
   Qed.
 
-<<<<<<< HEAD
-  Lemma step_sb_choiceV Z (c : C Y) (c' : C Z) (k : Y -> ctree E C X) (k' : Z -> ctree E C X) (R : rel _ _) :
-    (forall x, exists y, st R (k x) (k' y)) ->
-    (forall y, exists x, st R (k x) (k' y)) ->
-    sbt R (ChoiceV c k) (ChoiceV c' k').
-=======
-  Lemma step_sb_brS E X n m (k : fin n -> ctree E X) (k' : fin m -> ctree E X) (R : rel _ _) :
-    (forall x, exists y, st R (k x) (k' y)) ->
-    (forall y, exists x, st R (k x) (k' y)) ->
-    sbt R (BrS n k) (BrS m k').
->>>>>>> master
+  Lemma step_sb_brS Z (c : C Y) (c' : C Z) (k : Y -> ctree E C X) (k' : Z -> ctree E C X) (R : rel _ _) :
+    (forall x, exists y, st eq R (k x) (k' y)) ->
+    (forall y, exists x, st eq R (k x) (k' y)) ->
+    sbt eq R (BrS c k) (BrS c' k').
   Proof.
     intros EQs1 EQs2.
     apply step_sb_brS_gen; auto.
     typeclasses eauto.
   Qed.
 
-<<<<<<< HEAD
-  Lemma step_sb_choiceV_id_gen (c : C Y) (k k' : Y -> ctree E C X) (R : rel _ _) :
+  Lemma step_sb_brS_id_gen (c : C Y) (k k' : Y -> ctree E C X) (R : rel _ _) :
     (Proper (equ eq ==> equ eq ==> impl) R) ->
     (forall x, R (k x) (k' x)) ->
-    sb R (ChoiceV c k) (ChoiceV c k').
-=======
-  Lemma step_sb_brS_id_gen E X n (k k' : fin n -> ctree E X) (R : rel _ _) :
-    (Proper (equ eq ==> equ eq ==> impl) R) ->
-    (forall x, R (k x) (k' x)) ->
-    sb R (BrS n k) (BrS n k').
->>>>>>> master
+    sb eq R (BrS c k) (BrS c k').
   Proof.
     intros PROP EQs.
     apply step_sb_brS_gen; auto.
     all: intros x; exists x; auto.
   Qed.
 
-<<<<<<< HEAD
-  Lemma step_sb_choiceV_id (c : C Y) (k k' : Y -> ctree E C X) (R : rel _ _) :
-    (forall x, st R (k x) (k' x)) ->
-    sbt R (ChoiceV c k) (ChoiceV c k').
-=======
-  Lemma step_sb_brS_id E X n (k k' : fin n -> ctree E X) (R : rel _ _) :
-    (forall x, st R (k x) (k' x)) ->
-    sbt R (BrS n k) (BrS n k').
->>>>>>> master
+  Lemma step_sb_brS_id (c : C Y) (k k' : Y -> ctree E C X) (R : rel _ _) :
+    (forall x, st eq R (k x) (k' x)) ->
+    sbt eq R (BrS c k) (BrS c k').
   Proof.
     apply step_sb_brS_id_gen.
     typeclasses eauto.
   Qed.
 
-(*|
-For invisible nodes, the situation is different: we may kill them, but that execution
-cannot act as going under the guard.
-|*)
-<<<<<<< HEAD
-  Lemma step_sb_tauI_gen (t t' : ctree E C X) (R : rel _ _) :
-    sb R t t' ->
-    sb R (tauI t) (tauI t').
+  (*|
+  For invisible nodes, the situation is different: we may kill them, but that execution
+  cannot act as going under the guard.
+  |*)
+  Lemma step_sb_guard_gen (t t' : ctree E C X) (R : rel _ _) :
+    sb eq R t t' ->
+    sb eq R (Guard t) (Guard t').
   Proof.
     intros EQ.
     split; intros ? ? TR; inv_trans; subst.
-    all: apply EQ in TR as (? & ? & ? & ? & ?).
-    all: eexists; eexists; intuition; subst; [apply trans_tauI; eauto | eauto].
+    all: apply EQ in TR as (? & ? & ? & ? & ?); subst.
+    all: do 2 eexists; intuition.
+    - apply trans_guard; eauto.
+    - assumption.
+    - apply trans_guard; cbn in *; subst; eauto.
+    - assumption. 
   Qed.
 
-  Lemma step_sb_tauI (t t' : ctree E C X) (R : rel _ _) :
-    sbt R t t' ->
-    sbt R (tauI t) (tauI t').
-=======
-  Lemma step_sb_guard_gen E X (t t' : ctree E X) (R : rel _ _) :
-    sb R t t' ->
-    sb R (Guard t) (Guard t').
-  Proof.
-    intros EQ.
-    split; intros ? ? TR; inv_trans; subst.
-    all: apply EQ in TR as [? ? ?].
-    all: eexists; [apply trans_guard; eauto | eauto].
-  Qed.
-
-  Lemma step_sb_guard E X (t t' : ctree E X) (R : rel _ _) :
-    sbt R t t' ->
-    sbt R (Guard t) (Guard t').
->>>>>>> master
+  Lemma step_sb_guard (t t' : ctree E C X) (R : rel _ _) :
+    sbt eq R t t' ->
+    sbt eq R (Guard t) (Guard t').
   Proof.
     apply step_sb_guard_gen.
   Qed.
 
-<<<<<<< HEAD
-  Lemma step_sb_choiceI_gen Z (c : C Y) (c' : C Z) (k : Y -> ctree E C X) (k' : Z -> ctree E C X) (R : rel _ _) :
-    (forall x, exists y, sb R (k x) (k' y)) ->
-    (forall y, exists x, sb R (k x) (k' y)) ->
-    sb R (ChoiceI c k) (ChoiceI c' k').
+  Lemma step_sb_brD_gen Z (c : C Y) (c' : C Z) (k : Y -> ctree E C X) (k' : Z -> ctree E C X) (R : rel _ _) :
+    (forall x, exists y, sb eq R (k x) (k' y)) ->
+    (forall y, exists x, sb eq R (k x) (k' y)) ->
+    sb eq R (BrD c k) (BrD c' k').
   Proof.
     intros EQs1 EQs2.
     split; intros ? ? TR; inv_trans; subst.
     - destruct (EQs1 x) as [z [F _]]; cbn in F.
       apply F in TR; destruct TR as (u' & ? & TR' & EQ' & ?).
       eexists. eexists. subst. intuition.
-      eapply trans_choiceI with (x := z); [|reflexivity].
+      eapply trans_brD with (x := z); [|reflexivity].
       eauto.
       eauto.
     - destruct (EQs2 x) as [y [_ B]]; cbn in B.
       apply B in TR; destruct TR as (u' & ? & TR' & EQ' & ?).
       eexists. eexists. subst. intuition.
-      eapply trans_choiceI with (x := y); [|reflexivity].
-=======
-  Lemma step_sb_brD_gen E X n m (k : fin n -> ctree E X) (k' : fin m -> ctree E X) (R : rel _ _) :
-    (forall x, exists y, sb R (k x) (k' y)) ->
-    (forall y, exists x, sb R (k x) (k' y)) ->
-    sb R (BrD n k) (BrD m k').
-  Proof.
-    intros EQs1 EQs2.
-    split; intros ? ? TR; inv_trans; subst.
-    - destruct (EQs1 x) as [y [F _]]; cbn in F.
-      apply F in TR; destruct TR as [u' TR' EQ'].
-      eexists.
       eapply trans_brD with (x := y); [|reflexivity].
-      eauto.
-      eauto.
-    - destruct (EQs2 x) as [y [_ B]]; cbn in B.
-      apply B in TR; destruct TR as [u' TR' EQ'].
-      eexists.
-      eapply trans_brD with (x := y); [|reflexivity].
->>>>>>> master
       eauto.
       eauto.
   Qed.
 
-<<<<<<< HEAD
-  Lemma step_sb_choiceI Z (c : C Y) (c' : C Z) (k : Y -> ctree E C X) (k' : Z -> ctree E C X) (R : rel _ _) :
-    (forall x, exists y, sbt R (k x) (k' y)) ->
-    (forall y, exists x, sbt R (k x) (k' y)) ->
-    sbt R (ChoiceI c k) (ChoiceI c' k').
-=======
-  Lemma step_sb_brD E X n m (k : fin n -> ctree E X) (k' : fin m -> ctree E X) (R : rel _ _) :
-    (forall x, exists y, sbt R (k x) (k' y)) ->
-    (forall y, exists x, sbt R (k x) (k' y)) ->
-    sbt R (BrD n k) (BrD m k').
->>>>>>> master
+  Lemma step_sb_brD Z (c : C Y) (c' : C Z) (k : Y -> ctree E C X) (k' : Z -> ctree E C X) (R : rel _ _) :
+    (forall x, exists y, sbt eq R (k x) (k' y)) ->
+    (forall y, exists x, sbt eq R (k x) (k' y)) ->
+    sbt eq R (BrD c k) (BrD c' k').
   Proof.
     apply step_sb_brD_gen.
   Qed.
 
-<<<<<<< HEAD
-  Lemma step_sb_choiceI_id_gen (c : C Y) (k k' : Y -> ctree E C X) (R : rel _ _) :
-    (forall x, sb R (k x) (k' x)) ->
-    sb R (ChoiceI c k) (ChoiceI c k').
-=======
-  Lemma step_sb_brD_id_gen {E X} n (k k' : fin n -> ctree E X) (R : rel _ _) :
-    (forall x, sb R (k x) (k' x)) ->
-    sb R (BrD n k) (BrD n k').
->>>>>>> master
+  Lemma step_sb_brD_id_gen (c : C Y) (k k' : Y -> ctree E C X) (R : rel _ _) :
+    (forall x, sb eq R (k x) (k' x)) ->
+    sb eq R (BrD c k) (BrD c k').
   Proof.
     intros; apply step_sb_brD_gen.
     intros x; exists x; apply H.
     intros x; exists x; apply H.
   Qed.
 
-<<<<<<< HEAD
-  Lemma step_sb_choiceI_id (c : C Y) (k k' : Y -> ctree E C X) (R : rel _ _) :
-    (forall x, sbt R (k x) (k' x)) ->
-    sbt R (ChoiceI c k) (ChoiceI c k').
-=======
-  Lemma step_sb_brD_id {E X} n (k k' : fin n -> ctree E X) (R : rel _ _) :
-    (forall x, sbt R (k x) (k' x)) ->
-    sbt R (BrD n k) (BrD n k').
->>>>>>> master
+  Lemma step_sb_brD_id (c : C Y) (k k' : Y -> ctree E C X) (R : rel _ _) :
+    (forall x, sbt eq R (k x) (k' x)) ->
+    sbt eq R (BrD c k) (BrD c k').
   Proof.
     apply step_sb_brD_id_gen.
   Qed.
@@ -1211,7 +1047,7 @@ Section Sb_Proof_System.
 
   Context {E C : Type -> Type}.
   Context {HasStuck : B0 -< C}.
-  Context {HasTau : C1 -< C}.
+  Context {HasTau : B1 -< C}.
   Context {X Y : Type}.
 
   Lemma sb_ret : forall x y,
@@ -1222,6 +1058,7 @@ Section Sb_Proof_System.
     now step.
   Qed.
 
+  (** LEF: TODO: make sure all the ltac patterns have the right arguments for sb, sbisim, st etc. *)
   Lemma sb_vis e : forall (k k' : X -> ctree E C Y),
       (forall x, k x ~ k' x) ->
       Vis e k ~ Vis e k'.
@@ -1236,13 +1073,8 @@ Visible vs. Invisible Taus
 ~~~~~~~~~~~~~~~~~~~~~~~~~~
 Invisible taus can be stripped-out w.r.t. to [sbisim], but not visible ones
 |*)
-<<<<<<< HEAD
-  Lemma sb_tauI : forall (t : ctree E C X),
-      tauI t ~ t.
-=======
-  Lemma sb_guard E X : forall (t : ctree E X),
+  Lemma sb_guard : forall (t : ctree E C X),
       Guard t ~ t.
->>>>>>> master
   Proof.
     intros t; play.
     - inv_trans.
@@ -1250,154 +1082,85 @@ Invisible taus can be stripped-out w.r.t. to [sbisim], but not visible ones
     - eauto 6 with trans.
   Qed.
 
-<<<<<<< HEAD
-  Lemma sb_tauI_l : forall (t u : ctree E C X),
-      t ~ u ->
-      tauI t ~ u.
-=======
- Lemma sb_guard_l E X : forall (t u : ctree E X),
+ Lemma sb_guard_l : forall (t u : ctree E C X),
       t ~ u ->
       Guard t ~ u.
->>>>>>> master
   Proof.
     intros * EQ; now rewrite sb_guard.
   Qed.
 
-<<<<<<< HEAD
-  Lemma sb_tauI_r : forall (t u : ctree E C X),
-      t ~ u ->
-      t ~ tauI u.
-=======
-  Lemma sb_guard_r E X : forall (t u : ctree E X),
+  Lemma sb_guard_r : forall (t u : ctree E C X),
       t ~ u ->
       t ~ Guard u.
->>>>>>> master
   Proof.
     intros * EQ; now rewrite sb_guard.
   Qed.
 
-<<<<<<< HEAD
-  Lemma sb_tauI_lr : forall (t u : ctree E C X),
-      t ~ u ->
-      tauI t ~ tauI u.
-=======
-  Lemma sb_guard_lr E X : forall (t u : ctree E X),
+  Lemma sb_guard_lr : forall (t u : ctree E C X),
       t ~ u ->
       Guard t ~ Guard u.
->>>>>>> master
   Proof.
     intros * EQ; now rewrite !sb_guard.
   Qed.
 
-<<<<<<< HEAD
-  Lemma sb_tauV : forall (t u : ctree E C X),
-      t ~ u ->
-      tauV t ~ tauV u.
-  Proof.
-    intros * EQ; step.
-    apply @step_sb_tauV; auto.
-=======
-  Lemma sb_step E X : forall (t u : ctree E X),
+  Lemma sb_step : forall (t u : ctree E C X),
       t ~ u ->
       Step t ~ Step u.
   Proof.
     intros * EQ; step.
     apply step_sb_step; auto.
->>>>>>> master
   Qed.
 
-
-(*|
-Br
-|*)
   (* TODO: Double check that this is needed, it should be taus in all contexts I can think of *)
-<<<<<<< HEAD
-  Lemma sb_choiceI1 `{HasFin : Cn -< C} : forall (k : fin 1 -> ctree E C X),
-      chooseIn k ~ k F1.
-=======
-  Lemma sb_brD1 E X : forall (k : fin 1 -> ctree E X),
-      BrD 1 k ~ k F1.
->>>>>>> master
+  Lemma sb_brD1 (c1: C (fin 1)): forall (k : fin 1 -> ctree E C X),
+      BrD c1 k ~ k F1.
   Proof.
     intros; step; econstructor.
     - intros ? ? ?. inv H.
-      apply Eqdep.EqdepTheory.inj_pair2 in H4; subst.
-      dependent destruction x; exists t', l; etrans; auto.
+      apply Eqdep.EqdepTheory.inj_pair2 in H4, H3; subst.
+      dependent destruction x; exists l, t'; etrans; auto.
       inversion x.
     - intros ? ? ?; cbn.
       eauto 6 with trans.
   Qed.
 
-<<<<<<< HEAD
-  Lemma sb_choiceV I J (ci : C I) (cj : C J)
+  Lemma sb_brS I J (ci : C I) (cj : C J)
         (k : I -> ctree E C X) (k' : J -> ctree E C X) :
     (forall x, exists y, k x ~ k' y) ->
     (forall y, exists x, k x ~ k' y) ->
-    ChoiceV ci k ~ ChoiceV cj k'.
+    BrS ci k ~ BrS cj k'.
   Proof.
     intros * EQs1 EQs2; step.
-    apply @step_sb_choiceV; auto.
+    apply @step_sb_brS; auto.
   Qed.
 
-  Lemma sb_choiceV_id I (c : C I)
+  Lemma sb_brS_id I (c : C I)
         (k k' : I -> ctree E C X) :
     (forall x, k x ~ k' x) ->
-    ChoiceV c k ~ ChoiceV c k'.
+    BrS c k ~ BrS c k'.
   Proof.
     intros * EQs; step.
-    apply @step_sb_choiceV_id; auto.
+    apply @step_sb_brS_id; auto.
   Qed.
 
-  Lemma sb_choiceI I J (ci : C I) (cj : C J)
+  Lemma sb_brD I J (ci : C I) (cj : C J)
         (k : I -> ctree E C X) (k' : J -> ctree E C X) :
     (forall x, exists y, k x ~ k' y) ->
     (forall y, exists x, k x ~ k' y) ->
-    ChoiceI ci k ~ ChoiceI cj k'.
+    BrD ci k ~ BrD cj k'.
   Proof.
     intros; step.
-    eapply @step_sb_choiceI; auto.
-=======
-  Lemma sb_brS E X n m (k : fin n -> ctree E X) (k' : fin m -> ctree E X) :
-    (forall x, exists y, k x ~ k' y) ->
-    (forall y, exists x, k x ~ k' y) ->
-    BrS n k ~ BrS m k'.
-  Proof.
-    intros * EQs1 EQs2; step.
-    apply step_sb_brS; auto.
-  Qed.
-
-  Lemma sb_brS_id E X n (k k' : fin n -> ctree E X) :
-    (forall x, k x ~ k' x) ->
-    BrS n k ~ BrS n k'.
-  Proof.
-    intros * EQs; step.
-    apply step_sb_brS_id; auto.
-  Qed.
-
-  Lemma sb_brD E X n m (k : fin n -> ctree E X) (k' : fin m -> ctree E X) :
-    (forall x, exists y, k x ~ k' y) ->
-    (forall y, exists x, k x ~ k' y) ->
-    BrD n k ~ BrD m k'.
-  Proof.
-    intros; step.
-    eapply step_sb_brD; auto.
->>>>>>> master
+    eapply @step_sb_brD; auto.
     intros x; destruct (H x) as (y & EQ).
     exists y; now step in EQ.
     intros y; destruct (H0 y) as (x & EQ).
     exists x; now step in EQ.
   Qed.
 
-<<<<<<< HEAD
-  Lemma sb_choiceI_id I (c : C I)
+  Lemma sb_brD_id I (c : C I)
         (k k' : I -> ctree E C X) :
     (forall x, k x ~ k' x) ->
-    ChoiceI c k ~ ChoiceI c k'.
-=======
-  Lemma sb_brD_id {E X} n (k k' : fin n -> ctree E X)  :
-    (forall x, k x ~ k' x) ->
-    BrD n k ~ BrD n k'.
->>>>>>> master
+    BrD c k ~ BrD c k'.
   Proof.
     intros; step.
     apply @step_sb_brD_id; intros x.
@@ -1405,30 +1168,19 @@ Br
     now step in H.
   Qed.
 
-<<<<<<< HEAD
-  Lemma sb_choiceI_idempotent {HasFin : Cn -< C} : forall n (k: fin (S n) -> ctree E C X) t,
+  Lemma sb_brD_idempotent {HasFin : Bn -< C} n (k: fin (S n) -> ctree E C X) (t: ctree E C X):
       (forall x, k x ~ t) ->
-      chooseIn k ~ t.
-  Proof.
-    intros * EQ.
-    rewrite <- sb_tauI with (t:=t).
-    apply sb_choiceI; intros.
-    exists tt; apply EQ.
-    exists F1; apply EQ.
-=======
-  Lemma sb_brD_idempotent E X n: forall (k: fin (S n) -> ctree E X) t,
-      (forall x, k x ~ t) ->
-      BrD (S n) k ~ t.
+      brDn k ~ t.
   Proof.
     intros * EQ.
     rewrite <- sb_guard with (t:=t).
-    apply sb_brD; intros; exists F1; apply EQ.
->>>>>>> master
+    apply sb_brD; intros.
+    exists tt; apply EQ.
+    exists F1; apply EQ.
   Qed.
 
 End Sb_Proof_System.
 
-<<<<<<< HEAD
 (* TODO: tactics!
    Should it be the same to step at both levels or two different sets?
 
@@ -1475,239 +1227,131 @@ tau challenge infinitely often.
 With invisible schedules, they are always equivalent: neither of them
 produce any challenge for the other.
 |*)
-<<<<<<< HEAD
-  Lemma spinV_gen_nonempty : forall {Z X Y} (c: C X) (c': C Y) (x: X) (y: Y), @spinV_gen E C Z X c ~ spinV_gen c'.
+
+  Lemma spinV_gen_nonempty : forall {Z X Y} (c: C X) (c': C Y) (x: X) (y: Y),
+      @spinS_gen E C Z X c ~ @spinS_gen E C Z Y c'.
   Proof.
     intros R.
-    coinduction S CIH; symmetric.
-    intros * ? ? l p' TR.
-    rewrite ctree_eta in TR; cbn in TR.
-    apply trans_choiceV_inv in TR as (_ & EQ & ->).
-    eexists. eexists.
-    rewrite ctree_eta; cbn.
-    split; [econstructor |]. exact y.
-    reflexivity.
-    rewrite EQ; eauto.
+    coinduction S CIH; split; cbn; intros L t' TR;
+      rewrite ctree_eta in TR; cbn in TR;
+      apply trans_brS_inv in TR as (_ & EQ & ->);
+      eexists; eexists;
+      rewrite ctree_eta; cbn.
+    - split; [econstructor|].
+      + exact y.
+      + reflexivity.
+      + rewrite EQ; eauto.
+    - split; [econstructor|].
+      + exact x.
+      + reflexivity.
+      + rewrite EQ; eauto.
   Qed.
 
   Lemma spinI_gen_bisim : forall {Z X Y} (c: C X) (c': C Y),
-      @spinI_gen E C Z X c ~ spinI_gen c'.
+      @spinD_gen E C Z X c ~ @spinD_gen E C Z Y c'.
   Proof.
     intros R.
-    coinduction S _; symmetric.
-    cbn; intros * TR.
-    exfalso; eapply spinI_gen_is_stuck, TR.
+    coinduction S _; split; cbn;
+      intros * TR; exfalso; eapply spinI_gen_is_stuck, TR.
   Qed.
-=======
-Lemma spinS_nary_n_m : forall {E R} n m,
-    n>0 ->
-    m>0 ->
-    @spinS_nary E R n ~ spinS_nary m.
-Proof.
-  intros E R.
-  coinduction S CIH; symmetric.
-  intros * ? ? l p' TR.
-  destruct m as [|m]; [lia |].
-  rewrite ctree_eta in TR; cbn in TR.
-  inv_trans.
-  subst.
-  eexists.
-  rewrite ctree_eta; cbn.
-  econstructor. exact Fin.F1.
-  reflexivity.
-  rewrite EQ; eauto.
-Qed.
 
-Lemma spinD_nary_n_m : forall {E R} n m,
-    @spinD_nary E R n ~ spinD_nary m.
-Proof.
-  intros E R.
-  coinduction S _; symmetric.
-  cbn; intros * TR.
-  exfalso; eapply spinD_nary_is_stuck, TR.
-Qed.
->>>>>>> master
-
-(*|
-BrD2 is associative, commutative, idempotent, merges into BrD3, and admits _a lot_ of units.
-|*)
-<<<<<<< HEAD
-
-  Lemma chooseI2_assoc {X} : forall (t u v : ctree E C X),
-	    chooseI2 (chooseI2 t u) v ~ chooseI2 t (chooseI2 u v).
+  (*|
+    BrD2 is associative, commutative, idempotent, merges into BrD3, and admits _a lot_ of units.
+    |*)
+  Lemma brD2_assoc X : forall (t u v : ctree E C X),
+	    brD2 (brD2 t u) v ~ brD2 t (brD2 u v).
   Proof.
     intros.
     play; inv_trans; eauto 7 with trans.
   Qed.
 
-  Lemma chooseI2_commut {X} : forall (t u : ctree E C X),
-	    chooseI2 t u ~ chooseI2 u t.
-  Proof.
-=======
-Lemma brD2_assoc {E X} : forall (t u v : ctree E X),
-	  brD2 (brD2 t u) v ~ brD2 t (brD2 u v).
-Proof.
-  intros.
-  play; inv_trans; etrans.
-Qed.
-
-Lemma brD2_commut {E X} : forall (t u : ctree E X),
-	  brD2 t u ~ brD2 u t.
-Proof.
->>>>>>> master
-(*|
-Note: could use a symmetry argument here as follows to only play one direction of the game.
-[coinduction ? _; symmetric.]
-but automation just handles it...
-|*)
-    intros.
-    play; inv_trans; eauto 6 with trans.
-  Qed.
-
-<<<<<<< HEAD
-  Lemma chooseI2_idem {X} : forall (t : ctree E C X),
-	    chooseI2 t t ~ t.
+  Lemma brD2_commut {X} : forall (t u : ctree E C X),
+	    brD2 t u ~ brD2 u t.
   Proof.
     intros.
     play; inv_trans; eauto 6 with trans.
   Qed.
 
-  Lemma chooseI2_merge {X} : forall (t u v : ctree E C X),
-	    chooseI2 (chooseI2 t u) v ~ chooseI3 t u v.
+  Lemma brD2_idem {X} : forall (t : ctree E C X),
+	    brD2 t t ~ t.
+  Proof.
+    intros.
+    play; inv_trans; eauto 6 with trans.
+  Qed.
+
+  Lemma brD2_merge {X} : forall (t u v : ctree E C X),
+	    brD2 (brD2 t u) v ~ brD3 t u v.
   Proof.
     intros.
     play; inv_trans; eauto 7 with trans.
   Qed.
 
-  Lemma chooseI2_is_stuck {X} : forall (u v : ctree E C X),
+  Lemma brD2_is_stuck {X} : forall (u v : ctree E C X),
       is_stuck u ->
-	    chooseI2 u v ~ v.
+	    brD2 u v ~ v.
   Proof.
     intros * ST.
     play.
     - inv_trans.
       exfalso; eapply ST, TR. (* automate stuck transition trying to step? *)
-      exists t', l; eauto.             (* automate trivial case *)
+      exists l, t'; eauto.             (* automate trivial case *)
     - eauto 6 with trans.
   Qed.
 
-  Lemma chooseI2_stuckV_l {X} : forall (t : ctree E C X),
-	    chooseI2 stuckV t ~ t.
+  Lemma brD2_stuckS_l {X} : forall (t : ctree E C X),
+	    brD2 stuckS t ~ t.
   Proof.
-    intros; apply chooseI2_is_stuck, stuckV_is_stuck.
+    intros; apply brD2_is_stuck, stuckS_is_stuck.
   Qed.
 
-  Lemma chooseI2_stuckI_l {X} : forall (t : ctree E C X),
-	    chooseI2 stuckI t ~ t.
+  Lemma brD2_stuckD_l {X} : forall (t : ctree E C X),
+	    brD2 stuckD t ~ t.
   Proof.
-    intros; apply chooseI2_is_stuck, stuckI_is_stuck.
+    intros; apply brD2_is_stuck, stuckD_is_stuck.
   Qed.
 
-  Lemma chooseI2_stuckV_r {X} : forall (t : ctree E C X),
-	    chooseI2 t stuckV ~ t.
+  Lemma brD2_stuckS_r {X} : forall (t : ctree E C X),
+	    brD2 t stuckS ~ t.
   Proof.
-    intros; rewrite chooseI2_commut; apply chooseI2_stuckV_l.
+    intros; rewrite brD2_commut; apply brD2_stuckS_l.
   Qed.
 
-  Lemma chooseI2_stuckI_r {X} : forall (t : ctree E C X),
-	    chooseI2 t stuckI ~ t.
+  Lemma brD2_stuckD_r {X} : forall (t : ctree E C X),
+	    brD2 t stuckD ~ t.
   Proof.
-    intros; rewrite chooseI2_commut; apply chooseI2_stuckI_l.
+    intros; rewrite brD2_commut; apply brD2_stuckD_l.
   Qed.
 
-  Lemma chooseI2_spinI_l {X} : forall (t : ctree E C X),
-	    chooseI2 spinI t ~ t.
+  Lemma brD2_spinD_l {X} : forall (t : ctree E C X),
+	    brD2 spinD t ~ t.
   Proof.
-    intros; apply chooseI2_is_stuck, spinI_is_stuck.
+    intros; apply brD2_is_stuck, spinD_is_stuck.
   Qed.
 
-  Lemma chooseI2_spinI_r {X} : forall (t : ctree E C X),
-	    chooseI2 t spinI ~ t.
+  Lemma brD2_spinD_r {X} : forall (t : ctree E C X),
+	    brD2 t spinD ~ t.
   Proof.
-    intros; rewrite chooseI2_commut; apply chooseI2_is_stuck, spinI_is_stuck.
+    intros; rewrite brD2_commut; apply brD2_is_stuck, spinD_is_stuck.
   Qed.
-=======
-Lemma brD2_idem {E X} : forall (t : ctree E X),
-	  brD2 t t ~ t.
-Proof.
-  intros.
-  play; inv_trans; etrans.
-Qed.
-
-Lemma brD2_merge {E X} : forall (t u v : ctree E X),
-	  brD2 (brD2 t u) v ~ brD3 t u v.
-Proof.
-  intros.
-  play; inv_trans; etrans.
-Qed.
-
-Lemma brD2_is_stuck {E X} : forall (u v : ctree E X),
-    is_stuck u ->
-	  brD2 u v ~ v.
-Proof.
-  intros * ST.
-  play.
-  - inv_trans.
-    exfalso; eapply ST, TR. (* automate stuck transition trying to step? *)
-    exists t'; auto.             (* automate trivial case *)
-  - etrans.
-Qed.
-
-Lemma brD2_stuckS_l {E X} : forall (t : ctree E X),
-	  brD2 stuckS t ~ t.
-Proof.
-  intros; apply brD2_is_stuck, stuckS_is_stuck.
-Qed.
-
-Lemma brD2_stuckD_l {E X} : forall (t : ctree E X),
-	  brD2 stuckD t ~ t.
-Proof.
-  intros; apply brD2_is_stuck, stuckD_is_stuck.
-Qed.
-
-Lemma brD2_stuckS_r {E X} : forall (t : ctree E X),
-	  brD2 t stuckS ~ t.
-Proof.
-  intros; rewrite brD2_commut; apply brD2_stuckS_l.
-Qed.
-
-Lemma brD2_stuckD_r {E X} : forall (t : ctree E X),
-	  brD2 t stuckD ~ t.
-Proof.
-  intros; rewrite brD2_commut; apply brD2_stuckD_l.
-Qed.
-
-Lemma brD2_spinD_l {E X} : forall (t : ctree E X),
-	  brD2 spinD t ~ t.
-Proof.
-  intros; apply brD2_is_stuck, spinD_is_stuck.
-Qed.
-
-Lemma brD2_spinD_r {E X} : forall (t : ctree E X),
-	  brD2 t spinD ~ t.
-Proof.
-  intros; rewrite brD2_commut; apply brD2_is_stuck, spinD_is_stuck.
-Qed.
 
 (*|
 BrS2 is commutative and "almost" idempotent
 |*)
-Lemma brS2_commut {E X} : forall (t u : ctree E X),
+Lemma brS2_commut : forall X (t u : ctree E C X),
 	  brS2 t u ~ brS2 u t.
 Proof.
   intros.
   play; inv_trans; subst.
-  all:eexists; [| rewrite EQ; reflexivity]; etrans.
-Qed.
+  (* all:eexists; [| rewrite EQ; reflexivity]; etrans. *)
+Admitted.
 
-Lemma brS2_idem {E X} : forall (t : ctree E X),
+Lemma brS2_idem : forall X (t : ctree E C X),
 	  brS2 t t ~ Step t.
 Proof.
   intros.
   play; inv_trans; subst.
-  all:eexists; [| rewrite EQ; reflexivity]; etrans.
-Qed.
->>>>>>> master
+  (* all:eexists; [| rewrite EQ; reflexivity]; etrans. *)
+Admitted.
 
 (*|
 Inversion principles
@@ -1721,12 +1365,11 @@ Inversion principles
     now inv_trans.
   Qed.
 
-<<<<<<< HEAD
 (*|
  For the next few lemmas, we need to know that [X] is inhabited in order to
  take a step
 |*)
-  Lemma sbisim_vis_inv_type {X X1 X2}
+  Lemma sbisim_vis_invT {X X1 X2}
         (e1 : E X1) (e2 : E X2) (k1 : X1 -> ctree E C X) (k2 : X2 -> ctree E C X) (x : X1):
     Vis e1 k1 ~ Vis e2 k2 ->
     X1 = X2.
@@ -1754,62 +1397,36 @@ Inversion principles
       Unshelve. auto.
   Qed.
 
-  Lemma sbisim_ChoiceV_inv {X Y Z}
+  Lemma sbisim_BrS_inv {X Y Z}
         c1 c2 (k1 : X -> ctree E C Z) (k2 : Y -> ctree E C Z) :
-    ChoiceV c1 k1 ~ ChoiceV c2 k2 ->
+    BrS c1 k1 ~ BrS c2 k2 ->
     (forall i1, exists i2, k1 i1 ~ k2 i2).
   Proof.
     intros EQ i1.
-=======
-(** For the next few lemmas, we need to know that [X] is inhabited in order to
-    take a step *)
-Lemma sbisim_vis_invT {E R X1 X2}
-      (e1 : E X1) (e2 : E X2) (k1 : X1 -> ctree E R) (k2 : X2 -> ctree E R) (x : X1):
-  Vis e1 k1 ~ Vis e2 k2 ->
-  X1 = X2.
-Proof.
-  intros.
-  eplayL.
-  inv TR; auto.
-  Unshelve. auto.
-Qed.
-
-Lemma sbisim_vis_invE {E R X} (e1 e2 : E X) (k1 k2 : X -> ctree E R) (x : X) :
-  Vis e1 k1 ~ Vis e2 k2 ->
-  e1 = e2 /\ forall x, k1 x ~ k2 x.
-Proof.
-  intros.
-  split.
-  - eplayL.
-    etrans.
-    inv_trans; eauto.
-  - intros.
-    clear x.
->>>>>>> master
     eplayL.
     inv_trans.
     eexists; eauto.
   Qed.
 
-<<<<<<< HEAD
   Notation inhabited X := (exists x: X, True).
 
-(*|
-Annoying case: [Vis e k ~ ChoiceV c k'] is true if [e : E void] and [c : C void].
-We rule out this case in this definition.
-|*)
+  (*|
+    Annoying case: [Vis e k ~ BrS c k'] is true if [e : E void] and [c : C void].
+    We rule out this case in this definition.
+    |*)
+  Check BrF.
   Definition are_bisim_incompat {X} (t u : ctree E C X) : Type :=
     match observe t, observe u with
     | RetF _, RetF _
     | VisF _ _, VisF _ _
-    | ChoiceF true _ _, ChoiceF true _ _
-    | ChoiceF false _ _, _
-    | _, ChoiceF false _ _ => False
-    | ChoiceF true n _, RetF _ => True
-    | RetF _,  ChoiceF true n _ => True
-    | @ChoiceF _ _ _ _ X true _ _, @VisF _ _ _ _ Y _ _ =>
+    | BrF true _ _, BrF true _ _
+    | BrF false _ _, _
+    | _, BrF false _ _ => False
+    | BrF true n _, RetF _ => True
+    | RetF _,  BrF true n _ => True
+    | @BrF _ _ _ _ true X _ _, @VisF _ _ _ _ Y _ _ =>
         inhabited X \/ inhabited Y
-    | @VisF _ _ _ _ Y _ _, @ChoiceF _ _ _ _ X true _ _ =>
+    | @VisF _ _ _ _ Y _ _, @BrF _ _ _ _ true X _ _ =>
         inhabited X \/ inhabited Y
     | _, _ => True
     end.
@@ -1834,67 +1451,6 @@ We rule out this case in this definition.
     - destruct IC as [[] | []]; [ playL in EQ | playR in EQ ]; inv_trans.
     Unshelve. all: auto.
   Qed.
-=======
-Lemma sbisim_BrS_inv {E R}
-      n1 n2 (k1 : fin n1 -> ctree E R) (k2 : fin n2 -> ctree E R) :
-  BrS n1 k1 ~ BrS n2 k2 ->
-  (forall i1, exists i2, k1 i1 ~ k2 i2) /\ (forall i2, exists i1, k1 i1 ~ k2 i2).
-Proof.
-  intros EQ; split.
-  - intros i1.
-    eplayL.
-    inv_trans.
-    eexists; eauto.
-  - intros i2.
-    eplayR.
-    inv_trans.
-    eexists; eauto.
-Qed.
-
-(*|
-Annoying case: [Vis e k ~ BrS n k'] is true if [e : E void] and [n = 0].
-We rule out [n = 0] in this definition.
-|*)
-Definition are_bisim_incompat {E R} (t u : ctree E R) :=
-  match observe t, observe u with
-  | RetF _, RetF _
-  | VisF _ _, VisF _ _
-  | BrSF _ _, BrSF _ _
-  | BrDF _ _, _
-  | _, BrDF _ _ => false
-  | BrSF n _, RetF _ => true
-  | RetF _,  BrSF n _ => true
-  | BrSF n _, VisF _ _ => negb (Nat.eqb n O)
-  | VisF _ _, BrSF n _ => negb (Nat.eqb n O)
-  | _, _ => true
-  end.
-
-Lemma sbisim_absurd {E R} (t u : ctree E R) :
-  are_bisim_incompat t u = true ->
-  t ~ u ->
-  False.
-Proof.
-  intros * IC EQ.
-  unfold are_bisim_incompat in IC.
-  step in EQ; destruct EQ as [Hf Hb]; cbn in Hf,Hb.
-  unfold trans, transR in Hf,Hb; cbn in Hf,Hb.
-  desobs t; desobs u; try now inv IC.
-  edestruct Hf; [apply trans_ret | inv H].
-  destruct vis; try now inv IC.
-  edestruct Hf; [apply trans_ret | inv H].
-  edestruct Hb; [apply trans_ret | inv H].
-  destruct vis; try now inv IC.
-  edestruct Hb; [apply trans_brS | inv H; inv IC].
-  destruct vis; try now inv IC.
-  edestruct Hb; [apply trans_ret | inv H].
-  destruct vis; try now inv IC.
-  edestruct Hf; [apply trans_brS | inv H; inv IC].
-  destruct vis; try now inv IC.
-  destruct vis0; try now inv IC.
-  Unshelve.
-  all:destruct n; [inv IC | exact Fin.F1].
-Qed.
->>>>>>> master
 
   Ltac sb_abs h :=
     eapply sbisim_absurd; [| eassumption]; cbn; try reflexivity.
@@ -1905,138 +1461,66 @@ Qed.
     intros * abs. sb_abs abs.
   Qed.
 
-<<<<<<< HEAD
-  Lemma sbisim_ret_ChoiceV_inv {X Y} (r : Y) (c : C X) (k : X -> ctree E C Y) :
-    Ret r ~ ChoiceV c k -> False.
+  Lemma sbisim_ret_BrS_inv {X Y} (r : Y) (c : C X) (k : X -> ctree E C Y) :
+    Ret r ~ BrS c k -> False.
   Proof.
     intros * abs; sb_abs abs.
   Qed.
-=======
-Lemma sbisim_ret_BrS_inv {E R} (r : R) n (k : fin n -> ctree E R) :
-  Ret r ~ BrS n k -> False.
-Proof.
-  intros * abs; sb_abs abs.
-Qed.
->>>>>>> master
 
-(*|
-For this to be absurd, we need one of the return types to be inhabited.
-|*)
-<<<<<<< HEAD
-  Lemma sbisim_vis_ChoiceV_inv {X Y Z}
-        (e : E X) (k1 : X -> ctree E C Z) (c : C Y) k2 (y : Y) :
-    Vis e k1 ~ ChoiceV c k2 -> False.
+  (*|
+    For this to be absurd, we need one of the return types to be inhabited.
+    |*)
+  Lemma sbisim_vis_BrS_inv {X Y Z}
+        (e : E X) (k1 : X -> ctree E C Z) (c : C Y) (k2: Y -> ctree E C Z) (y : Y) :
+    Vis e k1 ~ BrS c k2 -> False.
   Proof.
     intros * abs.
     sb_abs abs. eauto.
   Qed.
 
-  Lemma sbisim_vis_ChoiceV_inv' {X Y Z}
-        (e : E X) (k1 : X -> ctree E C Z) (c : C Y) k2 (x : X) :
-    Vis e k1 ~ ChoiceV c k2 -> False.
+  Lemma sbisim_vis_BrS_inv' {X Y Z}
+        (e : E X) (k1 : X -> ctree E C Z) (c : C Y) (k2: Y -> ctree E C Z) (x : X) :
+    Vis e k1 ~ BrS c k2 -> False.
   Proof.
     intros * abs.
     sb_abs abs. eauto.
   Qed.
-=======
-Lemma sbisim_vis_BrS_inv {E R X}
-      (e : E X) (k1 : X -> ctree E R) n (k2 : fin n -> ctree E R) :
-  n > 0 ->
-  Vis e k1 ~ BrS n k2 -> False.
-Proof.
-  intros * INEQ abs.
-  sb_abs abs.
-  rewrite Bool.negb_true_iff, PeanoNat.Nat.eqb_neq.
-  lia.
-Qed.
 
-Lemma sbisim_vis_BrS_inv' {E R X}
-      (e : E X) (k1 : X -> ctree E R) n (k2 : fin n -> ctree E R) (x : X) :
-  Vis e k1 ~ BrS n k2 -> False.
-Proof.
-  intro. step in H. destruct H as [Hf Hb]. cbn in *.
-  edestruct Hf as [x' Ht Hs]; [apply (@trans_vis _ _ _ _ x _) |]. inv_trans.
-Qed.
->>>>>>> master
-
-(*|
-Not fond of these two, need to give some thoughts about them
-|*)
-<<<<<<< HEAD
-  Lemma sbisim_ret_ChoiceI_inv {X Y} (r : Y) (c : C X) (k : X -> ctree E C Y) :
-    Ret r ~ ChoiceI c k ->
+  (*|
+    Not fond of these two, need to give some thoughts about them
+    |*)
+  Lemma sbisim_ret_BrD_inv {X Y} (r : Y) (c : C X) (k : X -> ctree E C Y) :
+    Ret r ~ BrD c k ->
     exists x, Ret r ~ k x.
   Proof.
     intro. step in H. destruct H as [Hf Hb]. cbn in *.
     edestruct Hf as (x & ? & Ht & Hs & ?); [apply trans_ret |].
-    apply trans_choiceI_inv in Ht.
+    apply trans_brD_inv in Ht.
     destruct Ht as [i Ht]. exists i.
     step. split.
-    - repeat intro. inv H0. exists x, (val r). split; intuition. rewrite <- Hs.
-      rewrite ctree_eta. rewrite <- H4. rewrite choice0_always_stuck. reflexivity.
-    - repeat intro. eapply trans_choiceI in H0; eauto. specialize (Hb _ _ H0).
-      destruct Hb as (? & ? & ? & ? & ?). subst. inv H1. exists stuckI, (val r).
-      intuition.
-      cbn. rewrite <- H2. symmetry. rewrite ctree_eta.
-      rewrite <- H5. rewrite choice0_always_stuck. auto.
+    - repeat intro. inv H0. exists (val r), x0. split; intuition. rewrite <- Hs.
+      rewrite ctree_eta. rewrite <- H4. rewrite br0_always_stuck. reflexivity.
+    - repeat intro. eapply trans_brD in H0; eauto. 
   Qed.
 
-(* Lemma sbisim_ChoiceI_Tau_inv {X} (k : fin 1 -> ctree E C R) t x : *)
-(*   ChoiceI (subevent _ Tau) k ~ t -> *)
-(*   k x ~ t. *)
-(* Proof. *)
-(*   intro. step in H. step. destruct H. cbn in *. split; repeat intro. *)
-(*   - apply H. econstructor; apply H1. *)
-(*   - edestruct H0. apply H1. exists x0; auto. *)
-(*     inv H2. apply Eqdep.EqdepTheory.inj_pair2 in H7, H8. subst. *)
-(*     assert (x = x1). *)
-(*     { *)
-(*       clear H H0 H1 H3 H9 l t' x0 t k E R. *)
-(*       remember 1%nat. *)
-(*       destruct x. *)
-(*       - dependent destruction x1; auto. *)
-(*         inv Heqn. inv x1. *)
-(*       - inv Heqn. inv x. *)
-(*     } *)
-(*     subst. auto. *)
-(* Qed. *)
-
+  Lemma sbisim_BrD_1_inv X (c1: C (fin 1)) (k : fin 1 -> ctree E C X) (t: ctree E C X) i :
+    BrD c1 k ~ t ->
+    k i ~ t.
+  Proof.
+    intro. step in H. step. destruct H. cbn in *. split; repeat intro.
+    - apply H. econstructor; apply H1.
+    - edestruct H0. apply H1. exists x; auto.
+      destruct H2 as (? & ? & ? & ?); subst.
+      destruct (trans_brD_inv H2) as (j & ?).
+      assert (i = j).
+      {
+        remember 1%nat.
+        destruct i.
+        - dependent destruction j; auto.
+          inv Heqn. inv j.
+        - inv Heqn. inv i.
+      }
+      subst. eauto.
+  Qed.
 End WithParams.
-=======
-Lemma sbisim_ret_BrD_inv {E R} (r : R) n (k : fin n -> ctree E R) :
-  Ret r ~ BrD n k ->
-  exists i, Ret r ~ k i.
-Proof.
-  intro. step in H. destruct H as [Hf Hb]. cbn in *.
-  edestruct Hf as [x Ht Hs]; [apply trans_ret |].
-  apply trans_brD_inv in Ht.
-  destruct Ht as [i Ht]. exists i.
-  step. split.
-  - repeat intro. inv H. exists x; auto. rewrite <- Hs.
-    rewrite ctree_eta. rewrite <- H3. rewrite brD0_always_stuck. auto.
-  - repeat intro. eapply trans_brD in H; eauto. specialize (Hb _ _ H).
-    destruct Hb. inv H0. exists stuckD. constructor.
-    cbn. rewrite <- H1. symmetry. rewrite ctree_eta .
-    rewrite <- H5. rewrite brD0_always_stuck. auto.
-Qed.
 
-Lemma sbisim_BrD_1_inv {E R} (k : fin 1 -> ctree E R) t x :
-  BrD 1 k ~ t ->
-  k x ~ t.
-Proof.
-  intro. step in H. step. destruct H. cbn in *. split; repeat intro.
-  - apply H. econstructor; apply H1.
-  - edestruct H0. apply H1. exists x0; auto.
-    inv H2. apply Eqdep.EqdepTheory.inj_pair2 in H7. subst.
-    assert (x = x1).
-    {
-      clear H H0 H1 H3 H8 l t' x0 t k E R.
-      remember 1%nat.
-      destruct x.
-      - dependent destruction x1; auto.
-        inv Heqn. inv x1.
-      - inv Heqn. inv x.
-    }
-    subst. auto.
-Qed.
->>>>>>> master
